SystemFD.lean
@@ -1,3 +1,9 @@
 -- This module serves as the root of the `SystemFD` library.
 -- Import modules here that should be built as part of the library.
-import SystemFD.Basic
+import SystemFD.Algorithm.Soundness1
+import SystemFD.Algorithm.Soundness2
+-- import SystemFD.Evaluator.Soundness2
+import SystemFD.Examples.Boolean
+import SystemFD.Examples.Fundeps
+import SystemFD.Examples.Maybe
+import SystemFD.Examples.Nat
