SystemFD/Metatheory/Weaken.lean
@@ -2,10 +2,10 @@ import SystemFD.Term
 import SystemFD.Judgment
 import SystemFD.Ctx
 
--- theorem rename_lift r (A : Term) :
---   (∀ x, [r.to](Γ d@ x) = Δ d@ (r x)) ->
---   ∀ x, [r.lift.to]((A::Γ) d@ x) = ([r.to]A::Δ) d@ (Ren.lift r x)
--- := by
+theorem rename_lift r (A : Frame Term) :
+  (∀ x, (Γ d@ x).apply r.to = Δ d@ (r x)) ->
+  ∀ x, ((A::Γ) d@ x).apply r.lift.to = (A.apply r.to::Δ) d@ (Ren.lift r x)
+:= by sorry
 -- intro h x; simp
 -- cases x <;> simp at *
 -- case _ => rw [Subst.lift_lemma]; simp
@@ -24,9 +24,16 @@ theorem rename (r : Ren) :
   Judgment v Δ (idx_ren r idx)
 := by
 intro j wf h
-induction j <;> simp
+induction j generalizing Δ r <;> simp at *
 any_goals apply wf
-case _ Γ T t A j1 j2 ih1 ih2 => sorry
+case _ Γ T t A j1 j2 ih1 ih2 =>
+  replace ih2 := ih2 r wf h
+  have lem : ⊢ (Frame.datatype ([r.to]T) :: Δ) := by
+    constructor; apply ih2; apply wf
+  replace ih1 := @ih1 (Frame.datatype ([r.to]T) :: Δ) r.lift lem (rename_lift r (Frame.datatype T) h)
+  rw [Subst.lift_lemma] at ih1; simp at ih1
+  constructor; apply ih2; apply ih1
+case _ => sorry
 case _ => sorry
 case _ => sorry
 case _ => sorry
