SystemFD/Term/Substitution.lean
@@ -86,6 +86,7 @@ namespace Term
   | letdata t1 t2 => letdata (smap lf f t1) (smap lf (lf f) t2)
   | letterm t1 t2 t3 => letterm (smap lf f t1) (smap lf f t2) (smap lf (lf f) t3)
   | inst n t1 t2 => inst n (smap lf f t1) (smap lf (lf f) t2)
+  | decl t => decl (smap lf (lf f) t)
 end Term
 
 @[simp]
@@ -136,6 +137,9 @@ namespace Term
 
   @[simp]
   theorem subst_inst : [σ]inst n t1 t2 = inst n ([σ]t1) ([^σ]t2) := by unfold Subst.apply; simp
+
+  @[simp]
+  theorem subst_decl : [σ]decl t = decl ([^σ]t) := by unfold Subst.apply; simp
 
   theorem apply_id {t : Term} : [I]t = t := by
   have lem1 : ^I = @I Term := by
